WIP on generic recognizer optimized

src/Parsers/GenericRecognizerOptimized.v
@@ -7,18 +7,21 @@ Require Import Fiat.Parsers.ContextFreeGrammar.Core.
 Require Import Fiat.Parsers.ContextFreeGrammar.PreNotations.
 Require Import Fiat.Parsers.ContextFreeGrammar.Properties.
 Require Import Fiat.Parsers.ContextFreeGrammar.Carriers.
-Require Import Fiat.Parsers.BaseTypes.
+Require Import Fiat.Parsers.ContextFreeGrammar.SimpleCorrectness.
 Require Import Fiat.Parsers.GenericBaseTypes.
 Require Import Fiat.Parsers.GenericCorrectnessBaseTypes.
+Require Import Fiat.Parsers.BaseTypes.
 Require Import Fiat.Parsers.BaseTypesLemmas.
 Require Import Fiat.Parsers.CorrectnessBaseTypes.
 Require Import Fiat.Common Fiat.Common.Wf Fiat.Common.Wf2 Fiat.Common.Telescope.Core.
 Require Import Fiat.Parsers.GenericRecognizerExt.
+Require Import Fiat.Parsers.GenericRecognizer.
 Require Import Fiat.Parsers.GenericRecognizerCorrect.
-Require Import Fiat.Parsers.GenericRecognizerMin.
 Require Import Fiat.Parsers.Splitters.RDPList.
 Require Import Fiat.Parsers.ContextFreeGrammar.Valid.
 Require Import Fiat.Parsers.ContextFreeGrammar.ValidReflective.
+Require Import Fiat.Parsers.ContextFreeGrammar.Reflective.
+Require Import Fiat.Parsers.ContextFreeGrammar.ReflectiveLemmas.
 Require Import Fiat.Parsers.RecognizerPreOptimized.
 Require Import Fiat.Common.Match.
 Require Import Fiat.Common.List.ListFacts.
@@ -31,7 +34,7 @@ Require Export Fiat.Common.NatFacts.
 Require Export Fiat.Common.Sigma.
 Require Import Fiat.Parsers.StringLike.Core.
 Require Import Fiat.Parsers.StringLike.Properties.
-Require Import Fiat.Parsers.GenericRecognizer.
+Import NPeano.
 
 Set Implicit Arguments.
 Local Open Scope string_like_scope.
@@ -61,15 +64,17 @@ Module Export opt.
     Definition snd {A B} := Eval compute in @snd A B.
     Definition list_caset {A} := Eval compute in @list_caset A.
     Definition item_rect {A} := Eval compute in @item_rect A.
+    Definition ritem_rect {A} := Eval compute in @ritem_rect A.
     Definition bool_rect := Eval compute in bool_rect.
     Definition pred := Eval compute in pred.
     Definition minusr := Eval compute in minusr.
     Definition id {A} := Eval compute in @id A.
     Definition beq_nat := Eval compute in EqNat.beq_nat.
-    Definition leb := Eval compute in leb.
+    Definition leb := Eval compute in Compare_dec.leb.
+    Definition interp_RCharExpr {Char idata} := Eval cbv -[andb orb negb Compare_dec.leb] in @interp_RCharExpr Char idata.
   End opt.
 
-  Declare Reduction opt_red := cbv beta iota zeta delta [first_index_default map length uniquize string_beq option_rect up_to rev combine fold_left fold_right list_rect hd tl Common.opt.fst Common.opt.snd nth nth' fst snd list_caset item_rect bool_rect pred minusr id beq_nat leb].
+  Declare Reduction opt_red := cbv beta iota zeta delta [first_index_default map length uniquize string_beq option_rect up_to rev combine fold_left fold_right list_rect hd tl Common.opt.fst Common.opt.snd nth nth' fst snd list_caset item_rect ritem_rect bool_rect pred minusr id beq_nat leb interp_RCharExpr].
   Ltac opt_red x := eval opt_red in x.
 End opt.
 
@@ -95,15 +100,17 @@ Module Export opt2.
     Definition snd {A B} := Eval compute in @snd A B.
     Definition list_caset {A} := Eval compute in @list_caset A.
     Definition item_rect {A} := Eval compute in @item_rect A.
+    Definition ritem_rect {A} := Eval compute in @ritem_rect A.
     Definition bool_rect := Eval compute in bool_rect.
     Definition pred := Eval compute in pred.
     Definition minusr := Eval compute in minusr.
     Definition id {A} := Eval compute in @id A.
     Definition beq_nat := Eval compute in EqNat.beq_nat.
-    Definition leb := Eval compute in leb.
+    Definition leb := Eval compute in Compare_dec.leb.
+    Definition interp_RCharExpr {Char idata} := Eval cbv -[andb orb negb Compare_dec.leb] in @interp_RCharExpr Char idata.
   End opt2.
 
-  Declare Reduction opt2_red := cbv beta iota zeta delta [first_index_default map length uniquize string_beq option_rect up_to rev combine fold_left fold_right list_rect hd tl Common.opt.fst Common.opt.snd nth nth' fst snd list_caset item_rect bool_rect pred minusr id beq_nat leb].
+  Declare Reduction opt2_red := cbv beta iota zeta delta [first_index_default map length uniquize string_beq option_rect up_to rev combine fold_left fold_right list_rect hd tl Common.opt.fst Common.opt.snd nth nth' fst snd list_caset item_rect ritem_rect bool_rect pred minusr id beq_nat leb interp_RCharExpr].
   Ltac opt2_red x := eval opt2_red in x.
 End opt2.
 
@@ -129,39 +136,40 @@ Module Export opt3.
     Definition snd {A B} := Eval compute in @snd A B.
     Definition list_caset {A} := Eval compute in @list_caset A.
     Definition item_rect {A} := Eval compute in @item_rect A.
+    Definition ritem_rect {A} := Eval compute in @ritem_rect A.
     Definition bool_rect := Eval compute in bool_rect.
     Definition pred := Eval compute in pred.
     Definition minusr := Eval compute in minusr.
     Definition id {A} := Eval compute in @id A.
     Definition beq_nat := Eval compute in EqNat.beq_nat.
-    Definition leb := Eval compute in leb.
+    Definition leb := Eval compute in Compare_dec.leb.
+    Definition interp_RCharExpr {Char idata} := Eval cbv -[andb orb negb Compare_dec.leb] in @interp_RCharExpr Char idata.
   End opt3.
 
-  Declare Reduction opt3_red := cbv beta iota zeta delta [first_index_default map length uniquize string_beq option_rect up_to rev combine fold_left fold_right list_rect hd tl Common.opt.fst Common.opt.snd nth nth' fst snd list_caset item_rect bool_rect pred minusr id beq_nat leb].
+  Declare Reduction opt3_red := cbv beta iota zeta delta [first_index_default map length uniquize string_beq option_rect up_to rev combine fold_left fold_right list_rect hd tl Common.opt.fst Common.opt.snd nth nth' fst snd list_caset item_rect ritem_rect bool_rect pred minusr id beq_nat leb interp_RCharExpr].
   Ltac opt3_red x := eval opt3_red in x.
 End opt3.
 
 Section recursive_descent_parser.
   Context {Char} {HSLM : StringLikeMin Char} {HSL : StringLike Char}
-          {gendata : generic_parser_dataT Char}
-          {G : pregrammar' Char}.
+          {G : pregrammar Char}.
 
-  Let HNoDup' : NoDupR (fun x y => string_beq (fst x) (fst y)) (pregrammar_productions G).
+  (*Let HNoDup' : NoDupR (fun x y => string_beq (fst x) (fst y)) (pregrammar_productions G).
   Proof.
     pose proof (nonterminals_unique G) as HNoDup.
     hnf in HNoDup |- *; unfold pregrammar_nonterminals in *; simpl in *.
     rewrite uniquize_map in HNoDup.
     apply uniquize_length.
     apply (f_equal (@List.length _)) in HNoDup.
-    rewrite !map_length, uniquize_length in HNoDup.
-    rewrite HNoDup; reflexivity.
-  Qed.
+    rewrite !map_length in HNoDup.
+    rewrite !map_length, <- HNoDup; clear HNoDup.
+    reflexivity.
+  Qed.*)
 
   Context (Hvalid : is_true (grammar_rvalid G)).
 
   Let predata := @rdp_list_predata _ G.
   Local Existing Instance predata.
-  Context {gencdata : generic_parser_correctness_dataT}.
 
   Context {splitdata : @split_dataT Char _ _}.
 
@@ -174,72 +182,33 @@ Section recursive_descent_parser.
   Let rdata' : @parser_removal_dataT' _ G predata := rdp_list_rdata'.
   Local Existing Instance rdata'.
 
+  Context {gendata : generic_parser_dataT Char}
+          {gencdata : generic_parser_correctness_dataT}.
+
   Local Arguments minus !_ !_.
   Local Arguments min !_ !_.
 
-  Definition parse_nt_equiv str nt p1 p2
+  Let is_correct pnt str nt
     := forall b,
-      parse_nt_is_correct
-        (predata := predata)
-        str (@of_nonterminal _ data nt)
-        b
-        p1
-      <-> parse_nt_is_correct
-            (predata := predata)
-            str (@of_nonterminal _ optdata nt)
-            b
-            p2.
+      parse_nt_is_correct str (of_nonterminal nt) b pnt
+      <-> parse_nt_is_correct str (of_nonterminal nt) b (parse_nonterminal (data := data) str nt).
 
-  Global Instance parse_nt_equiv_Reflexive {str nt} : Reflexive (parse_nt_equiv str nt).
-  Proof. repeat intro; reflexivity. Qed.
-
-  Global Instance parse_nt_equiv_Symmetric {str nt} : Symmetric (parse_nt_equiv str nt).
-  Proof. repeat intro; symmetry; auto with nocore. Qed.
-
-  Global Instance parse_nt_equiv_Transitive {str nt} : Transitive (parse_nt_equiv str nt).
-  Proof. repeat intro; etransitivity; eauto with nocore. Qed.
-
-  Local Ltac t_parse_nt_equiv :=
-    lazymatch goal with
-    | [ H : ?R (bool_of_sum ?x) ?y,
-            H' : ?R (bool_of_sum ?x') ?y' |- parse_nt_equiv _ _ ?y ?y' ]
-      => intros [];
-         destruct x, x'; simpl @bool_of_sum in *
-    end;
-    repeat first [ assumption
-                 | progress simpl @bool_of_sum in *
-                 | progress simpl @of_nonterminal in *
-                 | progress simpl @BaseTypes.predata in *
-                 | progress unfold predata in *
-                 | split
-                 | intro
-                 | exfalso;
-                   solve [ eauto using @parse_nt_is_correct_disjoint with nocore ] ].
-
-  Lemma parse_nonterminal_optdata_correct
+  Lemma parse_nonterminal_optdata_eq
         {HSLP : StringLikeProperties Char}
         {splitdata_correct : @boolean_parser_completeness_dataT' _ _ _ G data}
         (str : String)
         (nt : String.string)
-    : parse_nt_equiv
-        str nt
-        (parse_nonterminal (data := optdata) str nt)
-        (parse_nonterminal (data := data) str nt).
+    : is_correct (parse_nonterminal (data := optdata) str nt) str nt.
   Proof.
     pose optsplitdata_correct.
-    pose proof (parse_nonterminal_correct (data := data) str nt).
-    pose proof (parse_nonterminal_correct (data := optdata) (cdata := optsplitdata_correct) str nt).
-    t_parse_nt_equiv.
-  Defined.
-
-  Local Ltac contract_drop_take_t' :=
-    idtac;
-    match goal with
-      | [ |- context[drop_takes_offset ?ls ?offset + ?v] ]
-        => change (drop_takes_offset ls offset + v) with (drop_takes_offset (drop_of v :: ls) offset)
-      | [ |- context[drop_takes_len ?ls ?len - ?v] ]
-        => change (drop_takes_len ls len - v) with (drop_takes_len (drop_of v :: ls) len)
-    end.
+    unfold is_correct.
+    pose proof (GenericRecognizerMin.parse_nonterminal_correct str nt).
+    pose proof (GenericRecognizerMin.parse_nonterminal_correct (cdata := optsplitdata_correct) str nt).
+    do 2 edestruct @GenericRecognizerMin.parse_nonterminal; simpl in *;
+      intros []; split; intro;
+        try solve [ tauto
+                  | exfalso; eauto using @parse_nt_is_correct_disjoint ].
+  Qed.
 
   Local Ltac contract_drop_take_t :=
     idtac;
@@ -253,10 +222,6 @@ Section recursive_descent_parser.
       | [ |- beq _ _ ] => reflexivity
       | [ |- Equivalence _ ] => split; repeat intro
     end.
-
-  Local Arguments drop_takes_offset : simpl never.
-  Local Arguments drop_takes_len : simpl never.
-  Local Arguments drop_takes_len_pf : simpl never.
 
   Local Ltac t_reduce_fix :=
     repeat match goal with
@@ -280,13 +245,13 @@ Section recursive_descent_parser.
                => apply f_equal3
              | _ => intro
              | [ |- ?x = ?x ] => reflexivity
-             | [ |- ret_nt _ = ret_nt _ ] => apply f_equal
-             | [ |- ret_production_cons _ _ = ret_production_cons _ _ ] => apply f_equal2
-             | [ |- ret_NonTerminal_true _ _ = ret_NonTerminal_true _ _ ] => apply f_equal2
              | [ |- bool_rect ?P _ _ ?b = bool_rect ?P _ _ ?b ] => apply f_equal3
              | [ |- andb _ _ = andb _ _ ] => apply f_equal2
              | [ |- andbr _ _ = andbr _ _ ] => apply f_equal2
              | [ |- orb _ _ = orb _ _ ] => apply f_equal2
+             | [ |- ret_nt _ = ret_nt _ ] => apply f_equal
+             | [ |- ret_NonTerminal_true _ _ = ret_NonTerminal_true _ _ ] => apply f_equal
+             | [ |- ret_production_cons _ _ = ret_production_cons _ _ ] => apply f_equal2
              | [ |- match ?it with Terminal _ => _ | _ => _ end = match ?it with _ => _ end ] => is_var it; destruct it
              | [ |- context[(fst ?x, snd ?x)] ] => rewrite <- !surjective_pairing
              | [ |- context[andb _ true] ] => rewrite Bool.andb_true_r
@@ -303,12 +268,6 @@ Section recursive_descent_parser.
              | [ |- context[orb false _] ] => rewrite Bool.orb_false_l
              | [ |- cons _ _ = cons _ _ ]
                => apply f_equal2
-             (*| _ => contract_drop_take_t'
-             | _ => rewrite make_drops_eta
-             | _ => rewrite make_drops_eta'
-             | _ => rewrite make_drops_eta''*)
-             (*| [ |- context[to_string (of_string _)] ] => rewrite !to_of*)
-             | _ => contract_drop_take_t'
              | _ => solve [ auto with nocore ]
              | [ |- prod_relation lt lt _ _ ] => hnf; simpl; omega
              | [ H : (_ && _)%bool = true |- _ ] => apply Bool.andb_true_iff in H
@@ -326,6 +285,8 @@ Section recursive_descent_parser.
                => destruct ls eqn:?
              | [ |- match ?ls with NonTerminal _ => _ | _ => _ end = match ?ls with _ => _ end ]
                => destruct ls eqn:?
+             | [ |- match ?ls with RNonTerminal _ => _ | _ => _ end = match ?ls with _ => _ end ]
+               => destruct ls eqn:?
              | [ |- (if ?e then _ else _) = (if ?e then _ else _) ]
                => destruct e eqn:?
              | _ => solve [ intuition ]
@@ -340,26 +301,26 @@ Section recursive_descent_parser.
 
   Local Ltac t_reduce_list :=
     idtac;
-    match goal with
-    | [ |- list_rect ?P ?n ?c ?ls ?idx ?offset ?len ?y = list_rect ?P' ?n' ?c' ?ls ?idx ?offset ?len ?y ]
+    lazymatch goal with
+    | [ |- list_rect ?P ?n ?c ?ls ?idx ?offset ?len = list_rect ?P' ?n' ?c' ?ls ?idx ?offset ?len ]
       => let n0 := fresh in
          let c0 := fresh in
          let n1 := fresh in
          let c1 := fresh in
          set (n0 := n);
-           set (n1 := n');
-           set (c0 := c);
-           set (c1 := c');
-           refine (list_rect
-                     (fun ls' => forall idx' l' y', list_rect P n0 c0 ls' idx' (drop_takes_offset l' offset) (drop_takes_len l' len) y' = list_rect P' n1 c1 ls' idx' (drop_takes_offset l' offset) (drop_takes_len l' len) y')
-                     _
-                     _
-                     ls
-                     idx
-                     nil y);
-           simpl list_rect;
-           [ subst n0 c0 n1 c1; cbv beta
-           | intros; unfold n0 at 1, c0 at 1, n1 at 1, c1 at 1 ]
+         set (n1 := n');
+         set (c0 := c);
+         set (c1 := c');
+         refine (list_rect
+                   (fun ls' => forall idx' offset' len', list_rect P n0 c0 ls' idx' offset' len' = list_rect P' n1 c1 ls' idx' offset' len')
+                   _
+                   _
+                   ls
+                   idx
+                   offset len);
+         simpl list_rect;
+         [ subst n0 c0 n1 c1; cbv beta
+         | intros; unfold c0 at 1, c1 at 1 ]
     end.
 
   Local Ltac t_reduce_list_generalize :=
@@ -414,28 +375,28 @@ Section recursive_descent_parser.
 
   Local Ltac refine_Fix2_5_Proper_eq_with_assumptions' HP HPpf :=
     idtac;
-    (lazymatch goal with
-      | [ |- context[@Fix2 ?A ?A' ?R ?Rwf ?T (fun a0 b0 c0 d0 e0 h0 i0 => @?f a0 b0 c0 d0 e0 h0 i0) ?a ?a' ?b ?c ?d ?e ?h] ]
-        => (lazymatch T with
-             | (fun a' : ?A0 => forall (b' :@?B a') (c' : @?C a' b') (d' : @?D a' b' c') (e' : @?E a' b' c' d') (h' : @?H a' b' c' d' e'), @?P a' b' c' d' e' h')
-               => let H' := fresh in
-                  pose proof ((fun f' H0 => @Fix2_5_Proper_eq_with_assumption A A' B C D E H R Rwf P HP f' f H0 a a' b c d e h HPpf)) as H';
-                  cbv beta in H';
-                  (lazymatch type of H' with
-                    | forall f' : ?f'T, @?H'T f' -> _
-                      => let H'' := fresh in
-                         let f'' := fresh in
-                         assert (H'' : { f' : f'T & H'T f' });
-                         [ clear H'
-                         | destruct H'' as [f'' H''];
-                           specialize (H' f'' H'');
-                           clear H''; eexists; symmetry; rewrite <- H' at 1; reflexivity ]
-                    end)
-             end)
-      end);
-    unfold forall_relation, pointwise_relation, respectful;
-    cbv beta;
-    eexists (fun a0 a0' b0 c0 d0 e0 h0 i0 => _); intros.
+      (lazymatch goal with
+        | [ |- context[_ = @Fix2 ?A ?A' ?R ?Rwf ?T (fun a0 b0 c0 d0 e0 h0 i0 => @?f a0 b0 c0 d0 e0 h0 i0) ?a ?a' ?b ?c ?d ?e ?h] ]
+          => (lazymatch T with
+               | (fun a' : ?A0 => forall (b' :@?B a') (c' : @?C a' b') (d' : @?D a' b' c') (e' : @?E a' b' c' d') (h' : @?H a' b' c' d' e'), @?P a' b' c' d' e' h')
+                 => let H' := fresh in
+                    pose proof ((fun f' H0 => @Fix2_5_Proper_eq_with_assumption A A' B C D E H R Rwf P HP f' f H0 a a' b c d e h HPpf)) as H';
+                    cbv beta in H';
+                    (lazymatch type of H' with
+                      | forall f' : ?f'T, @?H'T f' -> _
+                        => let H'' := fresh in
+                           let f'' := fresh in
+                           assert (H'' : { f' : f'T & H'T f' });
+                           [ clear H'
+                           | destruct H'' as [f'' H''];
+                             specialize (H' f'' H'');
+                             clear H''; eexists; exact H' ]
+                      end)
+               end)
+        end);
+      unfold forall_relation, pointwise_relation, respectful;
+      cbv beta;
+      eexists (fun a0 a0' b0 c0 d0 e0 h0 i0 => _); intros.
 
   Local Ltac refine_Fix2_5_Proper_eq_with_assumptions :=
     idtac;
@@ -451,7 +412,7 @@ Section recursive_descent_parser.
     let T := match type of HPpf with ?T -> _ => T end in
     let H0 := fresh "H" in
     assert (H0 : T)
-      by (simpl; unfold rdp_list_initial_nonterminals_data; rewrite map_length; reflexivity);
+      by (simpl; unfold rdp_list_initial_nonterminals_data, pregrammar'_of_pregrammar, pregrammar_productions; rewrite !map_length; reflexivity);
     let HPpf := constr:(HPpf H0) in
     refine_Fix2_5_Proper_eq_with_assumptions' HP HPpf.
 
@@ -459,6 +420,7 @@ Section recursive_descent_parser.
     repeat match goal with
              | [ |- _ = true ] => reflexivity
              | [ |- _ = false ] => reflexivity
+             | [ |- _ = ret_nt_invalid ] => reflexivity
              | [ |- ?x = ?x ] => reflexivity
              | [ |- _ = ?x ] => is_var x; reflexivity
              | [ |- _ = (_::_) ] => apply (f_equal2 (@cons _))
@@ -467,12 +429,13 @@ Section recursive_descent_parser.
              | [ |- _ = 1 ] => reflexivity
              | [ |- _ = None ] => reflexivity
              | [ |- _ = EqNat.beq_nat _ _ ] => apply f_equal2
-             | [ |- _ = leb _ _ ] => apply f_equal2
+             | [ |- _ = Compare_dec.leb _ _ ] => apply f_equal2
              | [ |- _ = S _ ] => apply f_equal
              | [ |- _ = string_beq _ _ ] => apply f_equal2
              | [ |- _ = fst ?x ] => is_var x; reflexivity
              | [ |- _ = snd ?x ] => is_var x; reflexivity
              | [ |- _ = pregrammar_productions ?x ] => is_var x; reflexivity
+             | [ |- _ = pregrammar_rproductions ?x ] => is_var x; reflexivity
              | [ |- context[(0 - _)%natr] ] => rewrite (minusr_minus 0); simpl (minus 0)
              | [ |- _ = (_, _) ] => apply f_equal2
              | _ => progress cbv beta
@@ -483,6 +446,22 @@ Section recursive_descent_parser.
              | [ |- context[andb _ false] ] => rewrite Bool.andb_false_r
              | [ |- context[andb _ true] ] => rewrite Bool.andb_true_r
            end.
+
+  Local Ltac misc_opt' :=
+    idtac;
+    match goal with
+    | _ => progress rewrite ?max_min_n, ?Minus.minus_diag, ?Nat.sub_0_r, ?uneta_bool, ?beq_nat_min_0(*, ?bool_rect_flatten*)
+    | _ => rewrite Min.min_l by assumption
+    | _ => rewrite Min.min_r by assumption
+    | [ |- context[if ?ltb ?x ?y then _ else _] ] => rewrite if_to_min
+    | [ |- context[min ?x ?y - ?x] ] => rewrite min_sub_same
+    | [ |- context[(min ?x ?y - ?x)%natr] ] => rewrite min_subr_same
+    | [ |- context[?x - (?x - ?y)%natr] ]
+      => rewrite !(minusr_minus x y), sub_twice, <- ?minusr_minus
+    | _ => progress fin_step_opt
+    end.
+
+  Local Ltac misc_opt := set_evars; progress repeat misc_opt'; subst_evars.
 
   Local Ltac step_opt' :=
     idtac;
@@ -560,6 +539,46 @@ Section recursive_descent_parser.
                       (fun c => item_rect T e1 e2 c = RHS c)
                       _ _);
             intro c; simpl @item_rect; subst e1 e2
+      | [ |- _ = ritem_rect ?T ?A ?B ?c ] (* evar kludge following *)
+        => revert c;
+          let RHS := match goal with |- forall c', _ = ?RHS c' => RHS end in
+          let f := constr:(fun TC NC =>
+                             forall c, ritem_rect T TC NC c = RHS c) in
+          let f := (eval cbv beta in f) in
+          let e1 := fresh in
+          let e2 := fresh in
+          match type of f with
+            | ?X -> ?Y -> _
+              => evar (e1 : X); evar (e2 : Y)
+          end;
+            intro c;
+            let ty := constr:(ritem_rect T e1 e2 c = RHS c) in
+            etransitivity_rev _; [ refine (_ : ty) | reflexivity ];
+            revert c;
+            refine (ritem_rect
+                      (fun c => ritem_rect T e1 e2 c = RHS c)
+                      _ _);
+            intro c; simpl @ritem_rect; subst e1 e2
+      | [ |- _ = match ?x with true => true | false => false end ]
+        => transitivity x; [ | destruct x; reflexivity ]
+      | [ |- _ = ret_nt _ ]
+        => refine (_ : ret_nt _ = _);
+           refine (f_equal ret_nt _)
+      | [ |- _ = ret_NonTerminal_true ?x _ ]
+        => refine (_ : ret_NonTerminal_true x _ = _);
+           refine (f_equal (ret_NonTerminal_true x) _)
+      | [ |- _ = fold_right ret_orb_productions ?init ?ls ]
+        => rewrite <- (rev_involutive ls), fold_left_rev_right
+      | [ |- _ = fold_right ret_orb_production ?init ?ls ]
+        => rewrite <- (rev_involutive ls), fold_left_rev_right
+      | [ |- _ = @fold_left ?A ?B ?orb _ ret_orb_productions_base ]
+        => refine (_ : fold_left orb _ ret_orb_productions_base = _);
+           apply (_ : Proper (_ ==> _ ==> _ ==> _) (@fold_left A B)); repeat intro
+      | [ |- _ = @fold_left ?A ?B ?orb _ ret_orb_production_base ]
+        => refine (_ : fold_left orb _ ret_orb_production_base = _);
+           apply (_ : Proper (_ ==> _ ==> _ ==> _) (@fold_left A B)); repeat intro
+      | [ |- _ = rev (map _ _) ]
+        => rewrite <- map_rev
     end;
     fin_step_opt.
 
@@ -568,12 +587,12 @@ Section recursive_descent_parser.
   Local Ltac sigL_transitivity term :=
     idtac;
     (lazymatch goal with
-    | [ |- ?sig (fun x : ?T => ?R (@?A x) ?B) ]
+    | [ |- ?sig (fun x : ?T => @?A x = ?B) ]
       => (let H := fresh in
           let H' := fresh in
-          assert (H : sig (fun x : T => R (A x) term));
+          assert (H : sig (fun x : T => A x = term));
           [
-          | assert (H' : R term B);
+          | assert (H' : term = B);
             [ clear H
             | let x' := fresh in
               destruct H as [x' H];
@@ -603,15 +622,24 @@ Section recursive_descent_parser.
 
   Local Ltac t_prereduce_list_evar :=
     idtac;
-    match goal with
-      | [ |- ?e = list_rect ?P (fun a b c d => _) (fun x xs H a b c d => _) ?ls ?A ?B ?C ?D ]
-        => refine (_ : list_rect P _ _ ls A B C D = _)
+    let RHS := match goal with |- _ = ?RHS => RHS end in
+    lazymatch RHS with
+    | appcontext RHS'[list_rect ?P ?f ?g]
+      => let ft := type of f in
+         let gt := type of g in
+         let f' := fresh in
+         let g' := fresh in
+         evar (f' : ft); evar (g' : gt);
+         let f0 := (eval unfold f' in f') in
+         let g0 := (eval unfold g' in g') in
+         let RHS'' := context RHS'[list_rect P f0 g0] in
+         refine (_ : RHS'' = _)
     end.
 
   Local Ltac t_postreduce_list :=
     idtac;
-    match goal with
-      | [ |- list_rect ?P ?N ?C ?ls ?a ?b ?c ?d = list_rect ?P ?N' ?C' ?ls ?a ?b ?c ?d ]
+    lazymatch goal with
+      | [ |- list_rect ?P ?N ?C ?ls ?a ?b ?c = list_rect ?P ?N' ?C' ?ls ?a ?b ?c ]
         => let P0 := fresh in
            let N0 := fresh in
            let C0 := fresh in
@@ -625,12 +653,12 @@ Section recursive_descent_parser.
              let IH := fresh "IH" in
              let xs := fresh "xs" in
              refine (list_rect
-                       (fun ls' => forall a' b' c' d',
-                                     list_rect P0 N0 C0 ls' a' b' c' d'
-                                     = list_rect P0 N1 C1 ls' a' b' c' d')
+                       (fun ls' => forall a' b' c',
+                                     list_rect P0 N0 C0 ls' a' b' c'
+                                     = list_rect P0 N1 C1 ls' a' b' c')
                        _
                        _
-                       ls a b c d);
+                       ls a b c);
                simpl @list_rect;
                [ subst P0 N0 C0 N1 C1; intros; cbv beta
                | intros ? xs IH; intros; unfold C0 at 1, C1 at 1; cbv beta;
@@ -645,7 +673,7 @@ Section recursive_descent_parser.
   Local Ltac t_postreduce_list_with_hyp :=
     idtac;
     match goal with
-      | [ |- list_rect ?P ?N ?C (?f ?a) ?a ?b ?c ?d = list_rect ?P ?N' ?C' (?f ?a) ?a ?b ?c ?d ]
+      | [ |- list_rect ?P ?N ?C (?f ?a) ?a ?b ?c = list_rect ?P ?N' ?C' (?f ?a) ?a ?b ?c ]
         => let P0 := fresh in
            let N0 := fresh in
            let C0 := fresh in
@@ -659,12 +687,12 @@ Section recursive_descent_parser.
              let IH := fresh "IH" in
              let xs := fresh "xs" in
              refine (list_rect
-                       (fun ls' => forall a' (pf : ls' = f a') b' c' d',
-                                     list_rect P0 N0 C0 ls' a' b' c' d'
-                                     = list_rect P0 N1 C1 ls' a' b' c' d')
+                       (fun ls' => forall a' (pf : ls' = f a') b' c',
+                                     list_rect P0 N0 C0 ls' a' b' c'
+                                     = list_rect P0 N1 C1 ls' a' b' c')
                        _
                        _
-                       (f a) a eq_refl b c d);
+                       (f a) a eq_refl b c);
                simpl @list_rect;
                [ subst P0 N0 C0 N1 C1; intros; cbv beta
                | intros ? xs IH; intros; unfold C0 at 1, C1 at 1; cbv beta;
@@ -684,7 +712,7 @@ Section recursive_descent_parser.
   Local Ltac t_postreduce_list_with_hyp_with_assumption :=
     idtac;
     lazymatch goal with
-      | [ H : ?HP (?HP' (?f ?a)) = true |- list_rect ?P ?N ?C (?f ?a) ?a ?b ?c ?d = list_rect ?P ?N' ?C' (?f ?a) ?a ?b ?c ?d ]
+      | [ H : ?HP (?HP' (?f ?a)) = true |- list_rect ?P ?N ?C (?f ?a) ?a ?b ?c = list_rect ?P ?N' ?C' (?f ?a) ?a ?b ?c ]
         => let P0 := fresh in
            let N0 := fresh in
            let C0 := fresh in
@@ -699,12 +727,12 @@ Section recursive_descent_parser.
              let xs := fresh "xs" in
              let pf := fresh "pf" in
              refine (list_rect
-                       (fun ls' => forall a' (pf : ls' = f a') (H' : HP (HP' (f a')) = true) b' c' d',
-                                     list_rect P0 N0 C0 ls' a' b' c' d'
-                                     = list_rect P0 N1 C1 ls' a' b' c' d')
+                       (fun ls' => forall a' (pf : ls' = f a') (H' : HP (HP' (f a')) = true) b' c',
+                                     list_rect P0 N0 C0 ls' a' b' c'
+                                     = list_rect P0 N1 C1 ls' a' b' c')
                        _
                        _
-                       (f a) a eq_refl H b c d);
+                       (f a) a eq_refl H b c);
                simpl @list_rect;
                [ subst P0 N0 C0 N1 C1; intros; cbv beta
                | intros ? xs IH pg; intros; unfold C0 at 1, C1 at 1; cbv beta;
@@ -712,7 +740,7 @@ Section recursive_descent_parser.
                    | [ |- appcontext[list_rect P0 N1 C1 ?ls'' ?a''] ]
                      => specialize (IH a'')
                  end;
-                 let T := match type of IH with ?T1 -> ?T2 -> _ => constr:(T1 * T2)%type end in
+                 let T := match type of IH with ?T1 -> ?T2 -> _ => constr:((T1 * T2)%type) end in
                  let H_helper := fresh in
                  let H_helper' := fresh in
                  assert (H_helper : T);
@@ -756,11 +784,14 @@ Section recursive_descent_parser.
           clear it; simpl @item_rect; intro))
     end).
 
-  Local Arguments leb !_ !_.
+  Local Arguments Compare_dec.leb !_ !_.
   Local Arguments to_nonterminal / .
 
   Local Instance good_nth_proper {A}
   : Proper (eq ==> _ ==> _ ==> eq) (nth (A:=A))
+    := _.
+  Local Instance good_nth'_proper {A}
+  : Proper (eq ==> _ ==> _ ==> eq) (nth' (A:=A))
     := _.
 
   Local Ltac rewrite_map_nth_rhs :=
@@ -835,6 +866,11 @@ Section recursive_descent_parser.
   Definition inner_nth' {A} := Eval unfold nth' in @nth' A.
   Definition inner_nth'_nth' : @inner_nth' = @nth'
     := eq_refl.
+
+  Local Instance good_inner_nth'_proper {A}
+  : Proper (eq ==> _ ==> _ ==> eq) (inner_nth' (A:=A))
+    := _.
+
 
   Lemma rdp_list_to_production_opt_sig x
   : { f : _ | rdp_list_to_production (G := G) x = f }.
@@ -926,65 +962,61 @@ Section recursive_descent_parser.
     rewrite minusr_minus; omega.
   Qed.
 
-  Section with_str.
-    Context (str : String)
-            (nt : String.string).
+  Definition parse_nonterminal_opt'0
+             (str : String)
+             (nt : String.string)
+  : { b : _ | b = parse_nonterminal (data := optdata) str nt }.
+  Proof.
+    exists (parse_nonterminal (data := optdata) str nt).
+    reflexivity.
+  Defined.
 
-    Local Infix "~=" := (parse_nt_equiv str nt).
-
-    Definition parse_nonterminal_opt'0
-      : { b : parse_nt_T | b ~= parse_nonterminal (data := optdata) str nt }.
-    Proof.
-      exists (parse_nonterminal (data := optdata) str nt).
-      reflexivity.
-    Defined.
-
-    Local Ltac optsplit_t' :=
-      idtac;
-      match goal with
+  Local Ltac optsplit_t' :=
+    idtac;
+    match goal with
       | [ |- _ = ?f match ?v with nil => ?N | x::xs => @?C x xs end ]
         => let RHS := match goal with |- _ = ?RHS => RHS end in
            let P := match (eval pattern v in RHS) with ?P _ => P end in
            transitivity (match v with
-                         | nil => P nil
-                         | x::xs => P (x::xs)
+                           | nil => P nil
+                           | x::xs => P (x::xs)
                          end);
-           [ simpl | destruct v; reflexivity ]
+             [ simpl | destruct v; reflexivity ]
       | [ |- _ = ?f match ?v with Terminal t => @?T t | NonTerminal nt => @?NT nt end ]
         => let RHS := match goal with |- _ = ?RHS => RHS end in
            let P := match (eval pattern v in RHS) with ?P _ => P end in
            transitivity (match v with
-                         | Terminal t => P (Terminal t)
-                         | NonTerminal nt => P (NonTerminal nt)
+                           | Terminal t => P (Terminal t)
+                           | NonTerminal nt => P (NonTerminal nt)
                          end);
-           [ simpl | destruct v; reflexivity ]
+             [ simpl | destruct v; reflexivity ]
       | [ |- ?e = match ?v with nil => ?N | x::xs => @?C x xs end :> ?T ]
         => idtac;
-           repeat match goal with
-                  | [ H : context[v] |- _ ]
-                    => hnf in H;
-                       match type of H with
-                       | context[v] => fail 1
-                       | _ => idtac
-                       end
-                  end;
-           let P := match (eval pattern v in T) with ?P _ => P end in
-           change (e = list_caset P N C v);
-           revert dependent v;
-           let NT := type of N in
-           let CT := type of C in
-           let N' := fresh in
-           let C' := fresh in
-           evar (N' : NT);
-           evar (C' : CT);
-           intro v; intros;
-           refine (_ : list_caset P N' C' v = list_caset P N C v);
-           refine (list_caset
-                     (fun v' => list_caset P N' C' v' = list_caset P N C v')
-                     _
-                     _
-                     v);
-           subst N' C'; simpl @list_caset; repeat intro
+          repeat match goal with
+                 | [ H : context[v] |- _ ]
+                   => hnf in H;
+                     match type of H with
+                     | context[v] => fail 1
+                     | _ => idtac
+                     end
+                 end;
+          let P := match (eval pattern v in T) with ?P _ => P end in
+          change (e = list_caset P N C v);
+            revert dependent v;
+            let NT := type of N in
+            let CT := type of C in
+            let N' := fresh in
+            let C' := fresh in
+            evar (N' : NT);
+              evar (C' : CT);
+              intro v; intros;
+              refine (_ : list_caset P N' C' v = list_caset P N C v);
+              refine (list_caset
+                        (fun v' => list_caset P N' C' v' = list_caset P N C v')
+                        _
+                        _
+                        v);
+              subst N' C'; simpl @list_caset; repeat intro
       | [ H : is_true (item_rvalid ?G ?v)
           |- ?e = match ?v with Terminal t => @?T t | NonTerminal nt => @?NT nt end ]
         => idtac; let TT := type of T in
@@ -992,99 +1024,98 @@ Section recursive_descent_parser.
                   let T' := fresh in
                   let NT' := fresh in
                   revert dependent v;
-                  evar (T' : TT);
-                  evar (NT' : NTT);
-                  intro v; intros;
-                  let eqP := match goal with |- _ = _ :> ?P => P end in
-                  let P := match (eval pattern v in eqP) with ?P _ => P end in
-                  change (e = item_rect P T NT v);
-                  refine (_ : item_rect P T' NT' v = item_rect P T NT v);
-                  refine (item_rect
-                            (fun v' => item_rvalid G v' -> item_rect P T' NT' v' = item_rect P T NT v')
-                            _
-                            _
-                            v H);
-                  subst T' NT';
-                  simpl @item_rect; intros ??
+                    evar (T' : TT);
+                    evar (NT' : NTT);
+                    intro v; intros;
+                    let eqP := match goal with |- _ = _ :> ?P => P end in
+                    let P := match (eval pattern v in eqP) with ?P _ => P end in
+                      change (e = item_rect P T NT v);
+                      refine (_ : item_rect P T' NT' v = item_rect P T NT v);
+                      refine (item_rect
+                                (fun v' => item_rvalid G v' -> item_rect P T' NT' v' = item_rect P T NT v')
+                                _
+                                _
+                                v H);
+                      subst T' NT';
+                      simpl @item_rect; intros ??
       | [ |- ?e = match ?v with Terminal t => @?T t | NonTerminal nt => @?NT nt end ]
         => idtac; let TT := type of T in
                   let NTT := type of NT in
                   let T' := fresh in
                   let NT' := fresh in
                   revert dependent v;
-                  evar (T' : TT);
-                  evar (NT' : NTT);
-                  intro v; intros;
-                  let eqP := match goal with |- _ = _ :> ?P => P end in
-                  let P := match (eval pattern v in eqP) with ?P _ => P end in
-                  change (e = item_rect P T NT v);
-                  refine (_ : item_rect P T' NT' v = item_rect P T NT v);
-                  refine (item_rect
-                            (fun v' => item_rect P T' NT' v' = item_rect P T NT v')
-                            _
-                            _
-                            v);
-                  subst T' NT';
-                  simpl @item_rect; intro
+                    evar (T' : TT);
+                    evar (NT' : NTT);
+                    intro v; intros;
+                    let eqP := match goal with |- _ = _ :> ?P => P end in
+                    let P := match (eval pattern v in eqP) with ?P _ => P end in
+                      change (e = item_rect P T NT v);
+                      refine (_ : item_rect P T' NT' v = item_rect P T NT v);
+                      refine (item_rect
+                                (fun v' => item_rect P T' NT' v' = item_rect P T NT v')
+                                _
+                                _
+                                v);
+                      subst T' NT';
+                      simpl @item_rect; intro
       | [ |- _ = _::_ ] => etransitivity_rev (_::_);
-                           [ apply f_equal2
-                           | reflexivity ]
+                          [ apply f_equal2
+                          | reflexivity ]
       | _ => progress fin_step_opt
-      end.
+    end.
 
-    Definition parse_nonterminal_opt'1
-      : { b : parse_nt_T | b ~= parse_nonterminal (data := optdata) str nt }.
-    Proof.
-      let c := constr:(parse_nonterminal_opt'0) in
-      let h := head c in
-      let p := (eval cbv beta iota zeta delta [proj1_sig h] in (proj1_sig c)) in
-      sigL_transitivity p; [ | abstract exact (proj2_sig c) ].
-      cbv beta iota zeta delta [parse_nonterminal parse_nonterminal' parse_nonterminal_or_abort list_to_grammar].
-      change (@parse_nonterminal_step Char) with (fun b c d e f g h i j k l => @parse_nonterminal_step Char b c d e f g h i j k l); cbv beta.
-      evar (b' : parse_nt_T).
-      sigL_transitivity b'; subst b';
-        [
-        | rewrite Fix5_2_5_eq by (intros; apply parse_nonterminal_step_ext; assumption);
-          reflexivity ].
-      simpl @fst; simpl @snd.
-      cbv beta iota zeta delta [parse_nonterminal parse_nonterminal' parse_nonterminal_or_abort parse_nonterminal_step parse_productions parse_productions' parse_production parse_item parse_item' Lookup list_to_grammar list_to_productions].
-      simpl.
-      cbv beta iota zeta delta [predata BaseTypes.predata initial_nonterminals_data nonterminals_length remove_nonterminal production_carrierT].
-      cbv beta iota zeta delta [rdp_list_predata Carriers.default_production_carrierT rdp_list_is_valid_nonterminal rdp_list_initial_nonterminals_data rdp_list_remove_nonterminal Carriers.default_nonterminal_carrierT rdp_list_nonterminals_listT rdp_list_production_tl Carriers.default_nonterminal_carrierT].
-      (*cbv beta iota zeta delta [rdp_list_of_nonterminal].*)
-      simpl; unfold pregrammar_nonterminals; simpl.
-      evar (b' : parse_nt_T).
-      sigL_transitivity b'; subst b';
-        [
-        | simpl;
-          rewrite !map_length, !length_up_to;
-          reflexivity ].
+  Local Ltac change_char_at_matches :=
+    idtac;
+    lazymatch goal with
+    | [ |- appcontext G[@char_at_matches ?Char ?HSLM ?n ?str (@interp_RCharExpr _ ?data ?P)] ]
+      => idtac;
+         let G' := context G[@char_at_matches_interp Char HSLM data n str P] in
+         change G'
+    end.
 
-      refine_Fix2_5_Proper_eq_with_assumptions.
-      etransitivity_rev _.
-      { fix2_trans_with_assumptions;
-        [
-        | unfold parse_production', parse_production'_for, parse_item', productions, production;
-          try solve [ t_reduce_fix;
-                      t_reduce_list;
-                      t_reduce_fix ] ].
+  Definition parse_nonterminal_opt'1
+             (str : String)
+             (nt : String.string)
+  : { b : _ | b = parse_nonterminal (data := optdata) str nt }.
+  Proof.
+    let c := constr:(parse_nonterminal_opt'0 str nt) in
+    let h := head c in
+    let p := (eval cbv beta iota zeta delta [proj1_sig h] in (proj1_sig c)) in
+    sigL_transitivity p; [ | abstract exact (proj2_sig c) ].
+    cbv beta iota zeta delta [parse_nonterminal GenericRecognizer.parse_nonterminal parse_nonterminal' GenericRecognizer.parse_nonterminal' parse_nonterminal_or_abort GenericRecognizer.parse_nonterminal_or_abort list_to_grammar].
+    simpl @GenericBaseTypes.parse_nt_T.
+    change (@GenericRecognizer.parse_nonterminal_step Char) with (fun b c d e f g h i j k l m => @GenericRecognizer.parse_nonterminal_step Char b c d e f g h i j k l m); cbv beta.
+    evar (b' : parse_nt_T).
+    sigL_transitivity b'; subst b';
+    [
+    | rewrite Fix5_2_5_eq by (intros; rapply (@parse_nonterminal_step_ext _ _ _ optdata _); assumption);
+      reflexivity ].
+    simpl @fst; simpl @snd.
+    cbv beta iota zeta delta [parse_nonterminal_step parse_productions parse_productions' parse_production parse_item parse_item' GenericRecognizer.parse_nonterminal_step GenericRecognizer.parse_productions GenericRecognizer.parse_productions' GenericRecognizer.parse_production GenericRecognizer.parse_item GenericRecognizer.parse_item' Lookup list_to_grammar list_to_productions].
+    simpl.
+    cbv beta iota zeta delta [predata BaseTypes.predata initial_nonterminals_data nonterminals_length remove_nonterminal production_carrierT].
+    cbv beta iota zeta delta [rdp_list_predata Carriers.default_production_carrierT rdp_list_is_valid_nonterminal rdp_list_initial_nonterminals_data rdp_list_remove_nonterminal Carriers.default_nonterminal_carrierT rdp_list_nonterminals_listT rdp_list_production_tl Carriers.default_nonterminal_carrierT].
+    (*cbv beta iota zeta delta [rdp_list_of_nonterminal].*)
+    simpl; unfold pregrammar_nonterminals; simpl.
+    evar (b' : parse_nt_T).
+    sigL_transitivity b'; subst b';
+    [
+    | simpl;
+      rewrite !map_length, !length_up_to;
+      reflexivity ].
+
+    refine_Fix2_5_Proper_eq_with_assumptions.
+    etransitivity_rev _.
+    { fix2_trans_with_assumptions;
+      [
+      | unfold parse_production', parse_production'_for, parse_item', GenericRecognizer.parse_production', GenericRecognizer.parse_production'_for, GenericRecognizer.parse_item', productions, production;
+        solve [ t_reduce_fix;
+                t_reduce_list;
+                t_reduce_fix ] ].
 
       (** Now we take advantage of the optimized splitter *)
       etransitivity_rev _.
-      { match goal with
-        | [ |- _ = option_rect ?P (fun x => _) ?N ?v ]
-          => refine (_ : option_rect P (fun x => _) N v = _)
-        end;
-        match goal with
-        | [ |- option_rect ?P ?S ?N ?v = option_rect ?P ?S' ?N' ?v ]
-          => refine (option_rect
-                       (fun v' => v = v' -> option_rect P S N v' = option_rect P S' N' v')
-                       (fun v' Hv => _)
-                       (fun Hv => _)
-                       v
-                       eq_refl);
-             simpl @option_rect
-        end; [ | reflexivity ].
+      { eapply option_rect_Proper_nondep_eq; [ intros ? Hv | reflexivity ].
         apply (f_equal (fun x => match x with Some _ => true | None => false end)) in Hv.
         simpl in Hv.
         lazymatch goal with
@@ -1102,8 +1133,6 @@ Section recursive_descent_parser.
               |- is_true (?R ?init ?nt) ]
             => apply H, H'
           end. }
-        step_opt'.
-        step_opt'.
         let nt := match type of Hvalid' with is_true (is_valid_nonterminal _ ?nt) => nt end in
         assert (Hvalid'' : productions_rvalid G (map to_production (nonterminal_to_production nt))).
         { unfold grammar_rvalid in Hvalid.
@@ -1115,15 +1144,25 @@ Section recursive_descent_parser.
         rewrite map_map in Hvalid''.
         pose proof (proj1 fold_right_andb_map_in_iff Hvalid'') as Hvalid'''.
         cbv beta in Hvalid'''.
+
+        misc_opt.
+        step_opt'.
+        step_opt'.
+        step_opt'.
+        step_opt'.
         apply map_Proper_eq_In; intros ? Hin.
+        apply in_rev in Hin.
         specialize (Hvalid''' _ Hin).
-        unfold parse_production', parse_production'_for.
+        unfold parse_production', parse_production'_for, GenericRecognizer.parse_production', GenericRecognizer.parse_production'_for.
         simpl.
+        (** Switch to using the list hypothesis, rather than lookup with the index *)
         etransitivity_rev _.
         { t_reduce_list_evar_with_hyp;
-          [ reflexivity
+          [
           |
           | ].
+          { step_opt'.
+            reflexivity. }
           { rewrite rdp_list_production_tl_correct.
             match goal with
               | [ H : _ = ?x |- context[?x] ]
@@ -1136,8 +1175,8 @@ Section recursive_descent_parser.
             reflexivity. } }
         (** Pull out the nil case once and for all *)
         etransitivity_rev _.
-        { match goal with
-            | [ |- _ = list_rect ?P ?N ?C (?f ?a) ?a ?b ?c ?d ]
+        { lazymatch goal with
+            | [ |- _ = list_rect ?P ?N ?C (?f ?a) ?a ?b ?c ]
               => let P0 := fresh in
                  let N0 := fresh in
                  let C0 := fresh in
@@ -1147,16 +1186,16 @@ Section recursive_descent_parser.
                    let IH := fresh "IH" in
                    let xs := fresh "xs" in
                    refine (list_rect
-                             (fun ls' => forall a' (pf : ls' = f a') b' c' d',
+                             (fun ls' => forall a' (pf : ls' = f a') b' c',
                                            (bool_rect
                                               (fun _ => _)
-                                              (N0 a' b' c' d')
-                                              (list_rect P0 (fun _ _ _ _ => true) C0 ls' a' b' c' d')
+                                              (N0 a' b' c')
+                                              (list_rect P0 (fun _ _ _ => ret_production_nil_true) C0 ls' a' b' c')
                                               (EqNat.beq_nat (List.length ls') 0))
-                                           = list_rect P0 N0 C0 ls' a' b' c' d')
+                                           = list_rect P0 N0 C0 ls' a' b' c')
                              _
                              _
-                             (f a) a eq_refl b c d);
+                             (f a) a eq_refl b c);
                      simpl @list_rect;
                      [ subst P0 N0 C0; intros; cbv beta
                      | intros ? xs IH; intros; unfold C0 at 1 3; cbv beta;
@@ -1178,30 +1217,27 @@ Section recursive_descent_parser.
                 => rewrite <- H; reflexivity
             end. }
           { simpl.
-            unfold parse_item'.
-            step_opt';
+            match goal with
+            | [ |- appcontext[EqNat.beq_nat (List.length ?ls) 0] ]
+              => is_var ls; destruct ls; simpl; try reflexivity
+            end; [].
             repeat match goal with
-                     | [ |- context[List.map _ match ?e with _ => _ end] ]
-                       => is_var e; destruct e
-                     | _ => progress simpl
-                     | [ |- ?x = ?x ] => reflexivity
-                     | _ => progress rewrite ?Bool.andb_true_r, ?Min.min_idempotent, ?Minus.minus_diag
-                     | [ H : EqNat.beq_nat _ _ = true |- _ ]
-                       => apply EqNat.beq_nat_true in H
-                     | _ => progress subst
-                     | [ |- context[EqNat.beq_nat ?x ?y] ]
-                       => is_var x; destruct (EqNat.beq_nat x y) eqn:?
-                     | [ H := _ |- _ ] => subst H
+                   | [ |- ?x = ?x ] => reflexivity
+                   | [ H := fun _ _ => _ |- _ ] => subst H; cbv beta
+                   | [ |- context[?x - (?y + (?x - ?y)) ] ]
+                     => replace (x - (y + (x - y))) with 0 by (clear; omega)
+                   | _ => rewrite minusr_minus
+                   | _ => progress simpl
                    end. } }
-        cbv beta.
-        step_opt'; [ | reflexivity ].
+        simpl.
+        step_opt'; [ reflexivity | | reflexivity ].
         etransitivity_rev _.
         { move Hvalid''' at bottom.
           simpl @to_production in Hvalid'''.
           unfold production_rvalid in Hvalid'''.
           t_prereduce_list_evar.
           t_postreduce_list_with_hyp_with_assumption;
-          [ reflexivity
+            [ reflexivity
             | let lem := constr:(production_tl_correct) in
               simpl rewrite lem;
               match goal with
@@ -1228,78 +1264,80 @@ Section recursive_descent_parser.
                    | _ => progress split_and
                    end. }
           etransitivity_rev _.
-          { step_opt'.
+          { do 4 step_opt'; [].
             etransitivity_rev _.
-            { repeat optsplit_t'.
-              { rewrite <- andbr_andb.
-                apply (f_equal2 andbr); [ | reflexivity ].
-                rewrite Min.min_idempotent at 2.
-                match goal with
-                  | [ |- _ = ?f ?b ?c ?d ?e ]
-                    => refine (f_equal (fun b' => f b' c d e) _)
-                end.
-                match goal with
-                  | [ |- _ = ?f (min ?x ?x) (?pf_f ?pf ?k) ]
-                    => etransitivity_rev (f x pf);
-                      [ generalize (pf_f pf k); rewrite Min.min_idempotent; intro
-                      | ]
-                end.
-                { f_equal; apply Le.le_proof_irrelevance. }
-                { reflexivity. } }
-              { apply (f_equal2 andb); [ | reflexivity ].
+            { step_opt'; [ reflexivity | ].
+              repeat optsplit_t'.
+              { reflexivity. }
+              { reflexivity. } }
+            unfold list_caset, item_rect.
+            repeat optsplit_t'.
+            { apply (f_equal2 ret_production_cons); [ | reflexivity ].
+              misc_opt.
+              rewrite Min.min_idempotent.
+              reflexivity. }
+            { apply (f_equal2 ret_production_cons).
+              { apply (f_equal3 (fun (b : bool) x y => if b then x else y)); [ | reflexivity | reflexivity ].
                 apply (f_equal2 andb); [ | reflexivity ].
                 match goal with
                 | [ |- _ = EqNat.beq_nat (min ?v ?x) ?v ]
                   => refine (_ : Compare_dec.leb v x = _)
                 end.
                 match goal with
-                | [ |- leb 1 ?x = _ ]
-                  => is_var x; destruct x as [|[|]]; try reflexivity
+                | [ |- Compare_dec.leb 1 ?x = _ ]
+                  => destruct x as [|[|]]; try reflexivity
                 end. }
-              { simpl in *.
-                match goal with
-                | [ H : is_true ?x |- context[?x] ] => rewrite H
-                end.
+              { rewrite !Nat.add_1_r.
                 reflexivity. } }
-            reflexivity. }
-          etransitivity_rev _.
-          { rewrite !(@fold_symmetric _ orb) by first [ apply Bool.orb_assoc | apply Bool.orb_comm ].
-            unfold parse_item'.
-            repeat optsplit_t'; repeat step_opt';
-              [ apply (f_equal2 andb) | ];
-              repeat optsplit_t'; repeat step_opt'.
-            { reflexivity. }
-            { reflexivity. }
             { simpl in *.
-              set_evars.
               match goal with
               | [ H : is_true ?x |- context[?x] ] => rewrite H
               end.
-              match goal with
-              | [ H := ?e |- _ ] => is_evar e; subst H
-              end.
-              reflexivity. }
-            { reflexivity. } }
+              reflexivity. } }
+          etransitivity_rev _.
+          { unfold parse_item', GenericRecognizer.parse_item'.
+            simpl.
+            repeat optsplit_t'; repeat step_opt';
+              [ apply (f_equal2 ret_production_cons) | ];
+              repeat optsplit_t'; try misc_opt; repeat step_opt'.
+          { reflexivity. }
+          { set_evars.
+            match goal with
+            | [ H : is_true ?x |- context[?x] ] => rewrite H
+            end.
+            match goal with
+            | [ H := ?e |- _ ] => is_evar e; subst H
+            end.
             reflexivity. }
-          reflexivity. }
+          { rewrite !minusr_minus, <- max_def, <- !minusr_minus.
+            reflexivity. }
+          { reflexivity. } }
+        reflexivity. }
+      reflexivity. }
 
-      unfold parse_production', parse_production'_for, parse_item', productions, production.
-      cbv beta iota zeta delta [predata BaseTypes.predata initial_nonterminals_data nonterminals_length remove_nonterminal production_carrierT].
-      cbv beta iota zeta delta [rdp_list_predata Carriers.default_production_carrierT rdp_list_is_valid_nonterminal rdp_list_initial_nonterminals_data rdp_list_remove_nonterminal Carriers.default_nonterminal_carrierT rdp_list_nonterminals_listT rdp_list_production_tl Carriers.default_nonterminal_carrierT].
+      progress unfold productions, production, rproductions, rproduction.
+      progress cbv beta iota zeta delta [rdp_list_predata Carriers.default_production_carrierT rdp_list_is_valid_nonterminal rdp_list_initial_nonterminals_data rdp_list_remove_nonterminal Carriers.default_nonterminal_carrierT rdp_list_nonterminals_listT rdp_list_production_tl Carriers.default_nonterminal_carrierT].
 
       step_opt'; [ | reflexivity ].
+      step_opt'.
       step_opt'.
       etransitivity_rev _.
       { cbv beta iota delta [rdp_list_nonterminal_to_production Carriers.default_production_carrierT Carriers.default_nonterminal_carrierT].
         simpl rewrite list_to_productions_to_nonterminal; unfold Lookup_idx.
         etransitivity_rev _.
         { step_opt'; [ reflexivity | ].
+          step_opt'.
           etransitivity_rev _.
           { step_opt'.
-            rewrite_map_nth_rhs; rewrite !map_map; simpl.
+            rewrite_map_nth_rhs; simpl; rewrite !map_map; simpl.
+            unfold interp_rproductions, interp_rproduction.
+            apply (f_equal2 (@nth _ _)); [ | reflexivity ].
+            step_opt'; [].
+            rewrite map_length.
             reflexivity. }
           rewrite_map_nth_dep_rhs; simpl.
           rewrite map_length.
+          unfold rproductions, rproduction.
           reflexivity. }
         rewrite_map_nth_rhs; rewrite !map_map; simpl.
         apply (f_equal2 (@nth _ _)); [ | reflexivity ].
@@ -1315,15 +1353,17 @@ Section recursive_descent_parser.
       reflexivity. }
     etransitivity_rev _.
     { etransitivity_rev _.
-      { repeat first [ idtac;
+      { repeat first [ rewrite uneta_bool
+                     | idtac;
                        match goal with
-                         | [ |- appcontext[@rdp_list_of_nonterminal] ] => fail 1
-                         | [ |- appcontext[@Carriers.default_production_tl] ] => fail 1
-                         | _ => reflexivity
+                       | [ |- appcontext[@rdp_list_of_nonterminal] ] => fail 1
+                       | [ |- appcontext[@Carriers.default_production_tl] ] => fail 1
+                       | _ => reflexivity
                        end
                      | step_opt'
                      | t_reduce_list_evar
                      | apply (f_equal2 andb)
+                     | apply (f_equal2 ret_production_cons)
                      | apply (f_equal2 (@cons _))
                      | t_refine_item_match ];
         first [ progress unfold rdp_list_of_nonterminal, Valid_nonterminals, grammar_of_pregrammar, pregrammar_nonterminals; simpl;
@@ -1331,8 +1371,8 @@ Section recursive_descent_parser.
                 reflexivity
               | idtac;
                 match goal with
-                  | [ |- _ = ?f ?A ?b ?c ?d ]
-                    => refine (f_equal (fun A' => f A' b c d) _)
+                  | [ |- _ = ?f ?A ?b ?c ]
+                    => refine (f_equal (fun A' => f A' b c) _)
                 end;
                 progress unfold Carriers.default_production_tl; simpl;
                 repeat step_opt'; [ reflexivity | ];
@@ -1350,7 +1390,8 @@ Section recursive_descent_parser.
               | idtac ].
         reflexivity. }
       etransitivity_rev _.
-      { repeat first [ idtac;
+      { set_evars.
+        repeat first [ idtac;
                        match goal with
                          | [ |- appcontext[@rdp_list_to_production] ] => fail 1
                          | _ => reflexivity
@@ -1358,9 +1399,11 @@ Section recursive_descent_parser.
                      | rewrite rdp_list_to_production_opt_correct
                      | step_opt'
                      | t_reduce_list_evar ].
+        subst_evars.
         reflexivity. }
       etransitivity_rev _.
       { step_opt'; [ | reflexivity ].
+        step_opt'.
         step_opt'.
         step_opt'.
         step_opt'; [ | reflexivity ].
@@ -1369,7 +1412,7 @@ Section recursive_descent_parser.
         etransitivity_rev _.
         { step_opt'.
           etransitivity_rev _.
-          { repeat step_opt'; [ | reflexivity ].
+          { repeat step_opt'; [ reflexivity | | reflexivity ].
             rewrite nth'_nth.
             rewrite_map_nth_rhs; rewrite !map_map; simpl.
             rewrite <- nth'_nth.
@@ -1379,7 +1422,15 @@ Section recursive_descent_parser.
             rewrite map_id.
             change @inner_nth' with @nth' at 3.
             rewrite nth'_nth.
+            unfold interp_rproductions, interp_rproduction, rproductions, rproduction, production.
+            rewrite !map_length.
+            progress repeat match goal with
+                            | [ |- appcontext[List.nth (@List.length ?B (@List.map ?A ?B ?f ?ls) - _)] ]
+                              => rewrite (@map_length A B f ls)
+                            end.
             rewrite_map_nth_rhs; simpl.
+            rewrite !map_map; simpl.
+            unfold productions, production.
             rewrite <- nth'_nth.
             change @nth' with @inner_nth'.
             apply f_equal2; [ | reflexivity ].
@@ -1393,11 +1444,15 @@ Section recursive_descent_parser.
             reflexivity. }
           etransitivity_rev _.
           { apply f_equal2; [ reflexivity | ].
-            rewrite bool_rect_andb; simpl.
-            rewrite Bool.andb_true_r.
+            lazymatch goal with
+            | [ |- _ = bool_rect ?P (if ?b then ?t else ?f) ?t ?b' ]
+              => transitivity (if (orb (negb b') b) then t else f); [ | destruct b, b'; reflexivity ]
+            end.
+            apply (f_equal3 (fun (b : bool) x y => if b then x else y)); [ | reflexivity | reflexivity ]. (*
             match goal with
-            | [ |- _ = (orb (negb (EqNat.beq_nat ?x 0)) (andb (EqNat.beq_nat ?x 0) ?y)) ]
-              => let z := fresh in
+            | [ |- context[negb (EqNat.beq_nat ?x 0)] ]
+              => replace (negb (EqNat.beq_nat x 0)) with (Compare_dec.leb
+let z := fresh in
                  let y' := fresh in
                  set (z := x);
                    set (y' := y);
@@ -1440,68 +1495,68 @@ Section recursive_descent_parser.
                        => progress unfold rdp_list_to_production_opt at 1; simpl;
                           change @inner_nth' with @nth';
                           repeat match goal with
-                                   | _ => progress simpl
-                                   | _ => progress fin_step_opt
-                                   | [ |- _ = @List.length ?A ?ls ]
-                                     => refine (f_equal (@List.length A) _)
-                                   | [ |- _ = nth' ?n ?ls ?d ]
-                                     => refine (f_equal2 (nth' n) _ _)
-                                   | [ |- _ = map (fun _ => nth' _ _ _) _ ]
-                                     => progress step_opt'
+                                 | _ => progress simpl
+                                 | _ => progress fin_step_opt
+                                 | _ => rewrite !map_length
+                                 | _ => rewrite !map_map
+                                 | _ => progress unfold interp_rproductions, interp_rproduction, rproductions, rproduction
+                                 | [ |- _ = nth' ?n ?ls ?d ]
+                                   => refine (f_equal2 (nth' n) _ _)
+                                 | [ |- _ = List.map _ (pregrammar_rproductions G) ]
+                                   => step_opt'
+                                 | [ |- _ = List.map (fun x : list (ritem _) => _) _ ]
+                                   => step_opt'
+                                 | _
+                                   => progress (rewrite nth'_nth;
+                                                progress rewrite_map_nth_rhs; rewrite !map_map; simpl;
+                                                rewrite <- nth'_nth)
+                                 | [ |- _ = List.length ?x ] => is_var x; reflexivity
                                  end;
-                          rewrite map_id;
                           fin_step_opt
                      end ];
       [ | reflexivity | reflexivity | ].
-      { t_reduce_list_evar; [ reflexivity | ].
-        repeat first [ step_opt'
-                     | apply (f_equal2 andb)
-                     | apply (f_equal2 andbr)
-                     | apply (f_equal3 char_at_matches)
-                     | progress fin_step_opt ].
-        { match goal with
-          | [ |- _ = ?f (?x - ?x) ?pf ]
-            => generalize pf;
-              rewrite Minus.minus_diag;
-              let pf' := fresh in
-              intro pf';
-                assert (Le.le_0_n _ = pf') by apply Le.le_proof_irrelevance;
-                subst pf'
-          end.
+      { rewrite list_rect_map.
+        t_reduce_list_evar; [ reflexivity | ].
+        set_evars.
+        setoid_rewrite list_caset_map.
+        unfold predata in *. (* work around bug #4673, https://coq.inria.fr/bugs/show_bug.cgi?id=4673 *)
+        setoid_rewrite item_rect_ritem_rect; cbv beta.
+        try setoid_rewrite uneta_bool.
+        subst_evars.
+
+        step_opt'; [].
+        step_opt'.
+        { set_evars.
+          setoid_rewrite combine_map_r.
+          do 2 setoid_rewrite map_map; simpl.
+          setoid_rewrite map_length.
+          progress change (fun x : ?A * ?B => fst x) with (@fst A B).
+          subst_evars.
+
           reflexivity. }
-        { reflexivity. }
-        { rewrite Plus.plus_comm; progress simpl.
-          match goal with
-            | [ |- _ = ?f (?x - ?y) (?pf ?a ?b ?c ?d) ]
-              => let f' := fresh in
-                 set (f' := f);
-                   let ty := constr:(f' (x - y)%natr (@opt_helper_minusr_proof a b c d) = f' (x - y) (pf a b c d )) in
-                   refine (_ : ty); change ty;
-                   clearbody f'
-          end.
-          match goal with
-            | [ |- ?f ?x ?y = ?f ?x' ?y' ]
-              => generalize y; generalize y'
-          end.
-          rewrite minusr_minus; intros; f_equal.
-          apply Le.le_proof_irrelevance. }
-        { reflexivity. }
-        { match goal with
-            | [ |- _ = ?f (?x - ?y) (?pf ?a ?b ?c ?d) ]
-              => let f' := fresh in
-                 set (f' := f);
-                   let ty := constr:(f' (x - y)%natr (@opt_helper_minusr_proof a b c d) = f' (x - y) (pf a b c d )) in
-                   refine (_ : ty); change ty;
-                   clearbody f'
-          end.
-          match goal with
-            | [ |- ?f ?x ?y = ?f ?x' ?y' ]
-              => generalize y; generalize y'
-          end.
-          rewrite minusr_minus; intros; f_equal.
-          apply Le.le_proof_irrelevance. }
-        { reflexivity. } }
+        { set_evars.
+          setoid_rewrite combine_map_r.
+          subst_evars.
+
+          step_opt'.
+          { set_evars.
+            do 2 setoid_rewrite map_map; simpl.
+            setoid_rewrite map_length.
+            rewrite !Nat.add_1_r.
+            subst_evars.
+
+            reflexivity. }
+          { step_opt'; [ | reflexivity ].
+            set_evars.
+            do 2 setoid_rewrite map_map; simpl.
+            setoid_rewrite map_length.
+            progress change (fun x : ?A * ?B => fst x) with (@fst A B).
+            subst_evars.
+
+            reflexivity. } } }
       { reflexivity. } }
+
+    simpl.
     reflexivity.
   Defined.
 
@@ -1523,7 +1578,7 @@ Section recursive_descent_parser.
                 change @inner_nth' with @nth';
                 t_reduce_fix;
                 t_postreduce_list;
-                unfold item_rect;
+                unfold ritem_rect;
                 t_reduce_fix ] ].
       reflexivity. }
 
@@ -1549,43 +1604,44 @@ Section recursive_descent_parser.
             step_opt'; [ | ].
             { rewrite nth'_nth.
               rewrite <- andbr_andb at 1.
-              apply (f_equal2 andbr); [ | reflexivity ].
-              match goal with
-              | [ |- _ = ?f ?x ?a ?b ?c ]
-                => refine (f_equal (fun x' => f x' a b c) _)
-              end.
-              fin_step_opt; [ reflexivity | ].
-              apply (f_equal2 (nth _)); [ | reflexivity ].
-              step_opt'; [ | reflexivity ].
-              rewrite nth'_nth; reflexivity. }
-            { step_opt'.
-              { rewrite <- andbr_andb at 1.
-                apply (f_equal2 andbr); [ reflexivity | ].
-                rewrite nth'_nth.
-                match goal with
-                | [ |- _ = ?f ?x ?a ?b ?c ]
-                  => refine (f_equal (fun x' => f x' a b c) _)
+              apply (f_equal2 andbr).
+              { match goal with
+                | [ |- _ = ?f ?x ?a ?b ]
+                  => refine (f_equal (fun x' => f x' a b) _)
                 end.
                 fin_step_opt; [ reflexivity | ].
                 apply (f_equal2 (nth _)); [ | reflexivity ].
                 step_opt'; [ | reflexivity ].
                 rewrite nth'_nth; reflexivity. }
               { step_opt'; [ | reflexivity ].
+                change_char_at_matches.
+                reflexivity. } }
+            { step_opt'.
+              { rewrite <- andbr_andb at 1.
+                apply (f_equal2 andbr); [ | ].
+                { change_char_at_matches.
+                  reflexivity. }
+                { rewrite nth'_nth.
+                  match goal with
+                  | [ |- _ = ?f ?x ?a ?b ]
+                    => refine (f_equal (fun x' => f x' a b) _)
+                  end.
+                  fin_step_opt; [ reflexivity | ].
+                  apply (f_equal2 (nth _)); [ | reflexivity ].
+                  step_opt'; [ | reflexivity ].
+                  rewrite nth'_nth; reflexivity. } }
+              { step_opt'; [ | reflexivity ].
                 apply (f_equal2 andb); [ reflexivity | ].
                 rewrite nth'_nth.
                 match goal with
-                | [ |- _ = ?f ?x ?a ?b ?c ]
-                  => refine (f_equal (fun x' => f x' a b c) _)
+                | [ |- _ = ?f ?x ?a ?b ]
+                  => refine (f_equal (fun x' => f x' a b) _)
                 end.
                 fin_step_opt; [ reflexivity | ].
                 apply (f_equal2 (nth _)); [ | reflexivity ].
                 step_opt'; [ | reflexivity ].
                 rewrite nth'_nth; reflexivity. } } }
-          { match goal with
-            | [ |- _ = @List.length ?A ?ls ]
-              => refine (f_equal (@List.length A) _)
-            end.
-            apply (f_equal2 (nth _)); [ | reflexivity ].
+          { apply (f_equal2 (nth _)); [ | reflexivity ].
             step_opt'; [ ].
             step_opt'; [ progress simpl ].
             rewrite nth'_nth.
@@ -1605,10 +1661,6 @@ Section recursive_descent_parser.
                    destruct z, y'; reflexivity
             end. }
           apply (f_equal2 orb); fin_step_opt; [].
-          match goal with
-          | [ |- _ = @List.length ?A ?ls ]
-            => refine (f_equal (@List.length A) _)
-          end.
           apply (f_equal2 (nth _)); [ | reflexivity ].
           step_opt'; [ ].
           step_opt'; [ progress simpl ].
@@ -1616,10 +1668,6 @@ Section recursive_descent_parser.
           apply (f_equal2 (nth _)); [ | reflexivity ].
           reflexivity. } }
       { apply (f_equal2 orb); fin_step_opt; [].
-        match goal with
-        | [ |- _ = @List.length ?A ?ls ]
-          => refine (f_equal (@List.length A) _)
-        end.
         apply (f_equal2 (nth _)); [ | reflexivity ].
         step_opt'; [ ].
         step_opt'; [ progress simpl ].
@@ -1743,14 +1791,17 @@ Section recursive_descent_parser.
     | [ |- context G[S (opt.id ?x)] ]
       => let G' := context G[opt.id (S x)] in
          change G'
-    | [ |- context G[leb (opt2.id ?x) (opt.id ?y)] ]
+    | [ |- context G[Compare_dec.leb (opt2.id ?x) (opt.id ?y)] ]
       => let G' := context G[opt2.id (opt2.leb x y)] in
          change G'
-    | [ |- context G[leb 1 (opt2.id ?x)] ]
+    | [ |- context G[Compare_dec.leb 1 (opt2.id ?x)] ]
       => let G' := context G[opt2.id (opt2.leb 1 x)] in
          change G'
-    | [ |- context G[leb 1 (opt2.length ?x)] ]
+    | [ |- context G[Compare_dec.leb 1 (opt2.length ?x)] ]
       => let G' := context G[opt2.id (opt2.leb 1 (opt2.length x))] in
+         change G'
+    | [ |- context G[@interp_RCharExpr ?Char ?idata (opt.id ?expr)] ]
+      => let G' := context G[opt.id (@opt.interp_RCharExpr Char idata expr)] in
          change G'
     end.
 
@@ -1803,6 +1854,7 @@ Section recursive_descent_parser.
     | [ |- _ = orbr _ _ ] => apply (f_equal2 orbr)
     | [ |- _ = andb _ _ ] => apply (f_equal2 andb)
     | [ |- _ = andbr _ _ ] => apply (f_equal2 andbr)
+    | [ |- _ = minusr _ _ ] => apply (f_equal2 minusr)
     | [ |- ?e = List.map ?f (opt2.id ?x) ]
       => progress change (e = opt2.map f x)
     | [ |- context G[List.map ?f (opt.id ?ls)] ]
@@ -1820,17 +1872,20 @@ Section recursive_descent_parser.
     | [ |- context G[item_rect ?x ?y ?z (opt.id ?w)] ]
       => let G' := context G[opt.id (opt.item_rect x y z w)] in
          change G'
+    | [ |- context G[ritem_rect ?x ?y ?z (opt.id ?w)] ]
+      => let G' := context G[opt.id (opt.ritem_rect x y z w)] in
+         change G'
     | [ |- context G[List.fold_left orb (opt.id ?ls) false] ]
       => let G' := context G[opt.id (opt.fold_left orb ls false)] in
          change G'
     | [ |- context G[List.fold_left orbr (opt.id ?ls) false] ]
       => let G' := context G[opt.id (opt.fold_left orbr ls false)] in
          change G'
-    | [ |- _ = list_rect ?P ?N ?C (opt.id ?ls) (opt2.id ?idx) ?offset ?len ?pf ]
+    | [ |- _ = list_rect ?P ?N ?C (opt.id ?ls) (opt2.id ?idx) ?offset ?len ]
       => t_reduce_list_evar;
         [
                | match goal with
-                 | [ |- ?e ?x ?xs ?H ?a ?b ?c ?d = _ ]
+                 | [ |- ?e ?x ?xs ?H ?a ?b ?c = _ ]
                    => is_evar e;
                      change x with (opt.id x);
                      change xs with (opt.id xs);
@@ -1857,6 +1912,27 @@ Section recursive_descent_parser.
                     _ _);
           intro c; simpl @opt.item_rect; subst e1 e2;
           change c with (opt.id c)
+    | [ |- _ = opt.ritem_rect ?T ?A ?B ?c ] (* evar kludge following *)
+      => revert c;
+        let RHS := match goal with |- forall c', _ = ?RHS c' => RHS end in
+        let f := constr:(fun TC NC =>
+                           forall c, opt.ritem_rect T TC NC c = RHS c) in
+        let f := (eval cbv beta in f) in
+        let e1 := fresh in
+        let e2 := fresh in
+        match type of f with
+        | ?X -> ?Y -> _
+          => evar (e1 : X); evar (e2 : Y)
+        end;
+          intro c;
+          let ty := constr:(opt.ritem_rect T e1 e2 c = RHS c) in
+          etransitivity_rev _; [ refine (_ : ty) | reflexivity ];
+          revert c;
+          refine (ritem_rect
+                    (fun c => opt.ritem_rect T e1 e2 c = RHS c)
+                    _ _);
+          intro c; simpl @opt.ritem_rect; subst e1 e2;
+          change c with (opt.id c)
     | [ |- _ = opt2.beq_nat _ _ ] => apply (f_equal2 opt2.beq_nat)
     | [ |- _ = opt2.leb _ _ ] => apply (f_equal2 opt2.leb)
     | [ |- _ = opt2.length _ ] => apply f_equal
@@ -1864,9 +1940,12 @@ Section recursive_descent_parser.
     | [ |- _ = opt2.snd _ ] => apply f_equal
     | [ |- _ = opt.fst _ ] => apply f_equal
     | [ |- _ = opt2.fst _ ] => apply f_equal
+    | [ |- _ = opt.interp_RCharExpr _ ] => apply f_equal
     | [ |- _ = opt.uniquize _ _ ] => reflexivity
     | [ |- _ = opt.combine _ _ ] => reflexivity
+    | [ |- _ = opt.length ?x ] => is_var x; reflexivity
     | [ |- _ = char_at_matches _ _ _ ] => apply f_equal3
+    | [ |- _ = char_at_matches_interp _ _ _ ] => apply f_equal3
     end.
 
   Local Ltac safe_change_opt := repeat safe_change_opt'.
@@ -1885,6 +1964,22 @@ Section recursive_descent_parser.
     repeat match goal with
            | [ flip_map := fun ls' f => @List.map _ _ f ls' |- _ ]
              => subst flip_map
+           end;
+    cbv beta.
+
+  Local Ltac do_flip_combine ls :=
+    idtac;
+    progress
+      (repeat let A := match goal with |- appcontext[@List.combine ?A ?B] => A end in
+              let B := match goal with |- appcontext[@List.combine A ?B] => B end in
+              let flip_combine := fresh "flip_combine" in
+              pose (flip_combine ls' f := @List.combine A B f ls');
+                progress change (@List.combine A B) with (fun f ls' => @flip_combine ls' f);
+                cbv beta;
+                try change (@flip_combine ls) with (@flip_combine (opt.id ls)));
+    repeat match goal with
+           | [ flip_combine := fun ls' f => @List.combine _ _ f ls' |- _ ]
+             => subst flip_combine
            end;
     cbv beta.
 
@@ -1929,10 +2024,12 @@ Section recursive_descent_parser.
                 change @opt2.map with @List.map;
                 t_reduce_fix;
                 t_postreduce_list;
-                unfold item_rect;
+                unfold ritem_rect;
                 t_reduce_fix ] ].
 
-      do_flip_map (pregrammar_productions G).
+      do_flip_map (pregrammar_rproductions G).
+      do_flip_combine (pregrammar_rproductions G).
+      change (List.length (pregrammar_rproductions G)) with (opt.id (opt.length (pregrammar_rproductions G))).
 
       step_opt'; [ | reflexivity ].
       apply (f_equal2 (opt3.nth' _)); [ | reflexivity ].
@@ -1940,8 +2037,8 @@ Section recursive_descent_parser.
       step_opt';
         change_opt_reduce; [ | | | ].
       { match goal with
-        | [ |- _ = ?f (opt2.id ?x) ?y ?z ?w ]
-          => refine (f_equal (fun x' => f x' y z w) _)
+        | [ |- _ = ?f (opt2.id ?x) ?y ?z ]
+          => refine (f_equal (fun x' => f x' y z) _)
         end.
         change_opt_reduce; [].
         match goal with
@@ -1949,13 +2046,13 @@ Section recursive_descent_parser.
           => unfold opt2.id; reflexivity
         end. }
       { match goal with
-        | [ |- _ = ?f _ _ _ (opt.id (opt.first_index_default _ _ _)) ]
+        | [ |- _ = ?f _ _ (opt.id (opt.first_index_default _ _ _)) ]
           => unfold opt.id
         end.
         reflexivity. }
       { match goal with
-        | [ |- _ = ?f (opt2.id ?x) ?y ?z ?w ]
-          => refine (f_equal (fun x' => f x' y z w) _)
+        | [ |- _ = ?f (opt2.id ?x) ?y ?z ]
+          => refine (f_equal (fun x' => f x' y z) _)
         end.
         change_opt_reduce; [].
         match goal with
@@ -1965,13 +2062,13 @@ Section recursive_descent_parser.
       { change @List.map with @opt2.map at 1. (** FIXME: is this right? *)
         change_opt_reduce; [ | | progress unfold opt2.id; reflexivity ].
         { match goal with
-          | [ |- _ = ?f _ _ _ (opt.id (opt.first_index_default _ _ _)) ]
+          | [ |- _ = ?f _ _ (opt.id (opt.first_index_default _ _ _)) ]
             => unfold opt.id
           end.
           reflexivity. }
         { match goal with
-          | [ |- _ = ?f (opt2.id ?x) ?y ?z ?w ]
-            => refine (f_equal (fun x' => f x' y z w) _)
+          | [ |- _ = ?f (opt2.id ?x) ?y ?z ]
+            => refine (f_equal (fun x' => f x' y z) _)
           end.
           change_opt_reduce; [].
           match goal with
@@ -1983,6 +2080,29 @@ Section recursive_descent_parser.
     reflexivity.
   Defined.
 
+  Definition parse_nonterminal_preopt
+             (str : String)
+             (nt : String.string)
+  : { b : bool | b = parse_nonterminal (data := optdata) str nt }.
+  Proof.
+    let c := constr:(parse_nonterminal_opt'2 str nt) in
+    let h := head c in
+    let impl := (eval cbv beta iota zeta delta [h proj1_sig] in (proj1_sig c)) in
+    (exists impl);
+      abstract (exact (proj2_sig c)).
+  Defined.
+
+  Lemma parse_nonterminal_preopt_eq
+        {HSLP : StringLikeProperties Char}
+        {splitdata_correct : @boolean_parser_completeness_dataT' _ _ _ G data}
+        (str : String)
+        (nt : String.string)
+    : proj1_sig (parse_nonterminal_preopt str nt) = parse_nonterminal (data := data) str nt.
+  Proof.
+    rewrite <- parse_nonterminal_optdata_eq.
+    apply proj2_sig.
+  Qed.
+
   Definition parse_nonterminal_opt
              (str : String)
              (nt : String.string)
@@ -1990,7 +2110,7 @@ Section recursive_descent_parser.
   Proof.
     let c := constr:(parse_nonterminal_opt'3 str nt) in
     let h := head c in
-    let impl := (eval cbv beta iota zeta delta [h proj1_sig item_rect list_caset] in (proj1_sig c)) in
+    let impl := (eval cbv beta iota zeta delta [h proj1_sig item_rect ritem_rect list_caset] in (proj1_sig c)) in
     (exists impl);
       abstract (exact (proj2_sig c)).
   Defined.
@@ -2006,3 +2126,4 @@ Section recursive_descent_parser.
     apply proj2_sig.
   Qed.
 End recursive_descent_parser.
+*)
